Treat receiver like other parameters in lit axioms
Previously, `this` was not treated like other parameters in the "lit axioms"
that allow function definitions to be expanded without consuming fuel in
the verifier. Perhaps that was okay before, we `this` was usually the same
in a recursive call. With type members for other types, like `datatype`,
a recursive function is likely to be called on something other than `this`.

In effect, this meant that the verifier could get stuck in infinite matching,
especially when faced with a false proof obligation (and in at least one
observed true proof obligation). The assertion in LitTriggers.dfy would
cause the verifier to never come back, but with this fix, the assertion is
quickly reported as an error.

This fix required `ThisExpr` nodes to be translated into Boogie AST nodes
with a filled-in type. Evidently, that was not needed before. For this reason,
this commit changed a number of calls to `ThisExpr` constructor.

Another parameter passed to Boogie functions is the heap. Since functions
do not change the heap, the heap parameter does not need to be lit-wrapped.
However, to reduce the chances that lit axioms will loop forever, dependencies
in the heap are disallowed--that is, if a function has a dependency on the
heap, it does not get lit axioms. This was done before. This could be improved
in two ways. (0) Checking an empty `reads` clause (which is what the code
does) does not detect dependencies on `const` fields. It is conceivable
that such dependencies could cause infinite matching of lit axioms, but I
have not seen any such example. (1) Instead of checking `reads` clauses,
perhaps the code could see if `decreases` expressions depend on the heap.
This would allow more examples to go through, and perhaps it could be done
without introducing infinite matching.

A final remark, the code previously had a special case: the nonemptiness of
the `reads` clause was ignored if the function signature contained an arrow
type. This let an example in TreeMapSimple.dfy go through. This special
case does not seem good, since the empty-`reads`-clause check can then
be subverted by introducing an unused arrow-typed parameter. So, I removed
this special case. I adjusted TreeMapSimple.dfy accordingly. Annoyingly, this
means the `TestY` assertion cannot be proved in `TestZ`--even with a manual
proof (because of lack of function extensionality, or as the case may be here,
lack of extensionality for functions with read effects).

Source/Dafny/Translator.cs
@@ -2524,8 +2524,7 @@ namespace Microsoft.Dafny {
       }
 
       // play havoc with the heap, except at the locations prescribed by (this._reads - this._modifies - {this})
-      var th = new ThisExpr(iter.tok);
-      th.Type = Resolver.GetThisType(iter.tok, iter);  // resolve here
+      var th = new ThisExpr(iter);  // resolve here
       var rds = new MemberSelectExpr(iter.tok, th, iter.Member_Reads);
       var mod = new MemberSelectExpr(iter.tok, th, iter.Member_Modifies);
       builder.Add(new Bpl.CallCmd(iter.tok, "$IterHavoc0",
@@ -2788,29 +2787,43 @@ namespace Microsoft.Dafny {
       sink.AddTopLevelDeclaration(ax);
       // TODO(namin) Is checking f.Reads.Count==0 excluding Valid() of BinaryTree in the right way?
       //             I don't see how this in the decreasing clause would help there.
-      // danr: Let's create the literal function axioms if there is an arrow type in the signature
       if (!(f is FixpointPredicate) && f.CoClusterTarget == Function.CoCallClusterInvolvement.None &&
-        (f.Reads.Count == 0 || f.Formals.Exists(a => a.Type.IsArrowType))) {
+        f.Reads.Count == 0 &&
+        !DafnyOptions.O.Dafnycc) {
         var FVs = new HashSet<IVariable>();
+        Type usesThis = null;
+        bool dontCare0 = false, dontCare1 = false;
+        var dontCareHeapAt = new HashSet<Label>();
         foreach (var e in f.Decreases.Expressions) {
-          ComputeFreeVariables(e, FVs);
+          ComputeFreeVariables(e, FVs, ref dontCare0, ref dontCare1, dontCareHeapAt, ref usesThis);
         }
+
+        var allFormals = new List<Formal>();
         var decs = new List<Formal>();
+        if (f.IsStatic) {
+          Contract.Assert(usesThis == null);
+        } else {
+          var surrogate = new ThisSurrogate(f.tok, Resolver.GetReceiverType(f.tok, f));
+          allFormals.Add(surrogate);
+          if (usesThis != null) {
+            decs.Add(surrogate);
+          }
+        }
         foreach (var formal in f.Formals) {
+          allFormals.Add(formal);
           if (FVs.Contains(formal)) {
             decs.Add(formal);
           }
         }
-        Contract.Assert(decs.Count <= f.Formals.Count);
-        if (0 < decs.Count && decs.Count < f.Formals.Count && !DafnyOptions.O.Dafnycc) {
+
+        Contract.Assert(decs.Count <= allFormals.Count);
+        if (0 < decs.Count && decs.Count < allFormals.Count) {
           ax = FunctionAxiom(f, body, decs);
           sink.AddTopLevelDeclaration(ax);
         }
 
-        if (!DafnyOptions.O.Dafnycc) {
-          ax = FunctionAxiom(f, body, f.Formals);
-          sink.AddTopLevelDeclaration(ax);
-        }
+        ax = FunctionAxiom(f, body, allFormals);
+        sink.AddTopLevelDeclaration(ax);
       }
     }
 
@@ -3014,7 +3027,11 @@ namespace Microsoft.Dafny {
       }
     }
 
-    Bpl.Axiom FunctionAxiom(Function f, Expression body, ICollection<Formal> lits, TopLevelDecl overridingClass = null) {
+    /// <summary>
+    /// The list of formals "lits" is allowed to contain an object of type ThisSurrogate, which indicates that
+    /// the receiver parameter of the function should be included among the lit formals.
+    /// </summary>
+    Bpl.Axiom FunctionAxiom(Function f, Expression body, List<Formal>/*?*/ lits, TopLevelDecl overridingClass = null) {
       Contract.Requires(f != null);
       Contract.Requires(predef != null);
       Contract.Requires(f.EnclosingClass != null);
@@ -3146,13 +3163,23 @@ namespace Microsoft.Dafny {
       }
 
       Bpl.Expr additionalAntecedent = null;
+      Expression receiverReplacement = null;
       if (!f.IsStatic) {
         var bvThis = new Bpl.BoundVariable(f.tok, new Bpl.TypedIdent(f.tok, etran.This, TrReceiverType(f)));
         forallFormals.Add(bvThis);
         funcFormals.Add(bvThis);
         reqArgs.Add(new Bpl.IdentifierExpr(f.tok, bvThis));
         var bvThisIdExpr = new Bpl.IdentifierExpr(f.tok, bvThis);
-        args.Add(bvThisIdExpr);
+        if (lits != null && lits.Exists(p => p is ThisSurrogate)) {
+          args.Add(Lit(bvThisIdExpr));
+          var th = new ThisExpr(f);
+          var l = new UnaryOpExpr(f.tok, UnaryOpExpr.Opcode.Lit, th) {
+            Type = th.Type
+          };
+          receiverReplacement = l;
+        } else {
+          args.Add(bvThisIdExpr);
+        }
         // add well-typedness conjunct to antecedent
         Type thisType = Resolver.GetReceiverType(f.tok, f);
         Bpl.Expr wh = Bpl.Expr.And(
@@ -3192,7 +3219,7 @@ namespace Microsoft.Dafny {
 
       Bpl.Expr pre = Bpl.Expr.True;
       foreach (MaybeFreeExpression req in f.Req) {
-        pre = BplAnd(pre, etran.TrExpr(Substitute(req.E, null, substMap)));
+        pre = BplAnd(pre, etran.TrExpr(Substitute(req.E, receiverReplacement, substMap)));
       }
       var preReqAxiom = pre;
       if (f is TwoStateFunction) {
@@ -3239,7 +3266,7 @@ namespace Microsoft.Dafny {
 
       // useViaCanCall: f#canCall(args)
       Bpl.IdentifierExpr canCallFuncID = new Bpl.IdentifierExpr(f.tok, f.FullSanitizedName + "#canCall", Bpl.Type.Bool);
-      Bpl.Expr useViaCanCall = new Bpl.NAryExpr(f.tok, new Bpl.FunctionCall(canCallFuncID), Concat(tyargs,args));
+      Bpl.Expr useViaCanCall = new Bpl.NAryExpr(f.tok, new Bpl.FunctionCall(canCallFuncID), Concat(tyargs, args));
 
       // ante := useViaCanCall || (useViaContext && typeAnte && pre)
       ante = Bpl.Expr.Or(useViaCanCall, ante);
@@ -3270,7 +3297,7 @@ namespace Microsoft.Dafny {
       if (!RevealedInScope(f) || (f.IsProtected && !InVerificationScope(f))) {
         tastyVegetarianOption = Bpl.Expr.True;
       } else {
-        var bodyWithSubst = Substitute(body, null, substMap);
+        var bodyWithSubst = Substitute(body, receiverReplacement, substMap);
         if (f is PrefixPredicate) {
           var pp = (PrefixPredicate)f;
           bodyWithSubst = PrefixSubstitution(pp, bodyWithSubst);
@@ -3308,7 +3335,7 @@ namespace Microsoft.Dafny {
         comment = "override axiom for " + f.FullSanitizedName + " in class " + overridingClass.FullSanitizedName;
       }
       if (lits != null) {
-        if (lits.Count == f.Formals.Count) {
+        if (lits.Count == f.Formals.Count + (f.IsStatic ? 0 : 1)) {
           comment += " for all literals";
         } else {
           comment += " for decreasing-related literals";
@@ -4747,10 +4774,9 @@ namespace Microsoft.Dafny {
       // body of 'C.F(this, x#0)'.
       // TODO:  More work needs to be done to support any type parameters that class C might have.  These would
       // need to be quantified (existentially?) in the axiom.
-      var receiver = new ThisExpr(f.tok);
-      receiver.Type = Resolver.GetReceiverType(f.tok, f);
+      var receiver = new ThisExpr(f);
       var args = f.OverriddenFunction.Formals.ConvertAll(p => (Expression)new IdentifierExpr(p.tok, p.Name) { Var = p, Type = p.Type });
-      var pseudoBody = new FunctionCallExpr(f.tok, f.Name, new ThisExpr(f.tok), f.tok, args);
+      var pseudoBody = new FunctionCallExpr(f.tok, f.Name, new ThisExpr(f), f.tok, args);
       pseudoBody.Function = f;  // resolve here
       // TODO: the following two lines (incorrectly) assume there are no type parameters
       pseudoBody.Type = f.ResultType;  // resolve here
@@ -5306,8 +5332,7 @@ namespace Microsoft.Dafny {
 
       // set up the information used to verify the method's modifies clause
       var iteratorFrame = new List<FrameExpression>();
-      var th = new ThisExpr(iter.tok);
-      th.Type = Resolver.GetThisType(iter.tok, iter);  // resolve here
+      var th = new ThisExpr(iter);
       iteratorFrame.Add(new FrameExpression(iter.tok, th, null));
       iteratorFrame.AddRange(iter.Modifies.Expressions);
       DefineFrame(iter.tok, iteratorFrame, builder, localVariables, null);
@@ -5567,7 +5592,7 @@ namespace Microsoft.Dafny {
       Contract.Requires(cce.NonNullElements(rw));
       Contract.Requires(substMap == null || cce.NonNullDictionaryAndValues(substMap));
       Contract.Requires(predef != null);
-      Contract.Requires(receiverReplacement == null || substMap != null);
+      Contract.Requires((substMap == null && receiverReplacement == null) || substMap != null);
       Contract.Ensures(Contract.Result<Bpl.Expr>() != null);
 
       // requires o to denote an expression of type RefType
@@ -5578,8 +5603,6 @@ namespace Microsoft.Dafny {
         Expression e = rwComponent.E;
         if (substMap != null) {
           e = Substitute(e, receiverReplacement, substMap);
-        } else {
-          Contract.Assert(receiverReplacement == null);
         }
 
         e = Resolver.FrameArrowToObjectSet(e, CurrentIdGenerator, program.BuiltIns);
@@ -8098,8 +8121,7 @@ namespace Microsoft.Dafny {
           SnocPrevH = xs => Snoc(xs, prevH);
         }
         if (f.IsStatic) {
-          // the value of 'selfExpr' won't be used, but it has to be non-null to satisfy the precondition of the call to InRWClause below
-          selfExpr = new ThisExpr(Token.NoToken);
+          selfExpr = null;
         } else {
           var selfTy = fromArrowType ? predef.HandleType : predef.RefType;
           var self = BplBoundVar("$self", selfTy, vars);
@@ -9895,8 +9917,7 @@ namespace Microsoft.Dafny {
           TrStmt(s.hiddenUpdate, builder, locals, etran);
         }
         // this.ys := this.ys + [this.y];
-        var th = new ThisExpr(iter.tok);
-        th.Type = Resolver.GetThisType(iter.tok, iter);  // resolve here
+        var th = new ThisExpr(iter);
         Contract.Assert(iter.OutsFields.Count == iter.OutsHistoryFields.Count);
         for (int i = 0; i < iter.OutsFields.Count; i++) {
           var y = iter.OutsFields[i];
@@ -10073,8 +10094,7 @@ namespace Microsoft.Dafny {
         AddComment(builder, stmt, "new;");
         fields.Iter(f => CheckDefiniteAssignmentSurrogate(s.SeparatorTok ?? s.EndTok, f, true, builder));
         fields.Iter(f => RemoveDefiniteAssignmentTrackerSurrogate(f));
-        var th = new ThisExpr(tok);
-        th.Type = Resolver.GetThisType(tok, cl);  // resolve here
+        var th = new ThisExpr(cl);
         var bplThis = (Bpl.IdentifierExpr)etran.TrExpr(th);
         SelectAllocateObject(tok, bplThis, th.Type, false, builder, etran);
         for (int i = 0; i < fields.Count; i++) {
@@ -10595,8 +10615,7 @@ namespace Microsoft.Dafny {
       Contract.Requires(builder != null);
       Contract.Requires(etran != null);
       // havoc Heap \ {this} \ _reads \ _new;
-      var th = new ThisExpr(tok);
-      th.Type = Resolver.GetThisType(tok, iter);  // resolve here
+      var th = new ThisExpr(iter);
       var rds = new MemberSelectExpr(tok, th, iter.Member_Reads);
       var nw = new MemberSelectExpr(tok, th, iter.Member_New);
       builder.Add(new Bpl.CallCmd(tok, "$YieldHavoc",
@@ -14294,7 +14313,7 @@ namespace Microsoft.Dafny {
           }
 
         } else if (expr is ThisExpr) {
-          return new Bpl.IdentifierExpr(expr.tok, This);
+          return new Bpl.IdentifierExpr(expr.tok, This, translator.TrType(expr.Type));
 
         } else if (expr is IdentifierExpr) {
           IdentifierExpr e = (IdentifierExpr)expr;
@@ -18376,7 +18395,7 @@ namespace Microsoft.Dafny {
     {
       ISet<string> namesToAvoid = new HashSet<string>();
       public AlphaConverting_Substituter(Expression receiverReplacement, Dictionary<IVariable, Expression> substMap, Dictionary<TypeParameter, Type> typeMap)
-        : base(receiverReplacement is ImplicitThisExpr ? new ThisExpr(receiverReplacement.tok) : receiverReplacement, substMap, typeMap) {
+        : base(receiverReplacement is ImplicitThisExpr ? new ThisExpr(receiverReplacement.tok) { Type = receiverReplacement.Type } : receiverReplacement, substMap, typeMap) {
         Contract.Requires(substMap != null);
         Contract.Requires(typeMap != null);
       }
